huge progress

FunnyLang/AST.lean
@@ -23,6 +23,33 @@ def NEList.toList : NEList α → List α
   | uno  a   => [a]
   | cons a b => a :: b.toList
 
+def NEList.concat : NEList α → α → NEList α
+  | cons a b, x => cons a $ concat b x
+  | uno  a,   x => cons a $ uno x
+
+def NEList.append (l : NEList α) : NEList α → NEList α
+  | cons a b => l.concat a |>.append b
+  | uno  a   => l.concat a
+
+theorem NEListToListEqListOfNonEmpty {l : List α} [BEq α] (h : ¬ l.isEmpty) :
+    (l.toNEList h).toList = l := by
+  induction l with
+  | nil         => simp only [List.isEmpty] at h
+  | cons _ t hi =>
+    by_cases he : List.isEmpty t
+    · have : t = [] := by
+        match t with
+        | []     => rfl
+        | _ :: _ => simp only [List.isEmpty] at he
+      simp only [this, NEList.toList]
+    · simp only [NEList.toList, List.toNEList, he, hi he]
+
+/-! # TODO
+Similarly, prove theorems about `concat` and `append`, using the implementations
+from `List` as the ground truth and the back and forth translations between
+`List` and `NEList`.
+-/
+
 def List.unfoldStrings (l : List String) : String :=
   l.foldl (init := "") $ fun acc a => acc ++ s!" {a}" |>.trimLeft
 
@@ -61,7 +88,7 @@ mutual
     | ifElse      : Expression → Program → Program → Program
     | whileLoop   : Expression → Program → Program
     | evaluation  : Expression → Program
-    | err         : String     → Program
+    | fail        : String     → Program
     deriving Inhabited, Repr
 
 end
@@ -73,107 +100,172 @@ def Program.getCurryNames? : Program → Option (NEList String)
   | sequence (attribution _ (evaluation (atom (curry ns _)))) _ => some ns
   | _                                                           => none
 
-def nSpacesAux (cs : List Char) : Nat → List Char
+def Program.isSequence : Program → Bool
+  | sequence .. => true
+  | _           => false
+
+def blankAux (cs : List Char) : Nat → List Char
   | 0     => cs
-  | n + 1 => ' ' :: ' ' :: cs
+  | n + 1 => ' ' :: ' ' :: (blankAux cs n)
 
-def nSpaces (n : Nat) : String :=
-  ⟨nSpacesAux [] n⟩
-
-def Program.lengthAux (n : Nat) : Program → Nat
-  | Program.sequence _ q => q.lengthAux (n + 1)
-  | _ => n + 1
-
-def Program.length (p : Program) : Nat :=
-  p.lengthAux 0
+def blank (n : Nat) : String :=
+  ⟨blankAux [] n⟩
 
 mutual
 
   partial def valToString : Value → String
-    | nil => "nil"
-    | Value.bool b => toString b
-    | int i => toString i
-    | float f => toString f
-    | list l => toString $ l.map fun v => valToString v
-    | str s => s
+    | nil       => "nil"
+    | .bool b   => toString b
+    | int   i   => toString i
+    | float f   => toString f
+    | list  l   => toString $ l.map fun v => valToString v
+    | str   s   => s
     | curry _ p => progToString p
-    | error s => s
+    | error s   => s!"error: {s}"
 
   partial def unfoldExpressions (es : NEList Expression) : String :=
     (es.toList.map fun e => expToString e).unfoldStrings
 
   partial def expToString : Expression → String
-    | atom v => valToString v
-    | var n  => n
-    | Expression.not e => s!"(! {expToString e})"
-    | add l r => s!"({expToString l} + {expToString r})"
-    | mul l r => s!"({expToString l} * {expToString r})"
-    | app n es => s!"{n} {unfoldExpressions es}"
-    | eq l r => s!"({expToString l} = {expToString r})"
-    | ne l r => s!"({expToString l} != {expToString r})"
-    | lt l r => s!"({expToString l} < {expToString r})"
-    | le l r => s!"({expToString l} <= {expToString r})"
-    | gt l r => s!"({expToString l} > {expToString r})"
-    | ge l r => s!"({expToString l} >= {expToString r})"
+    | atom v    => valToString v
+    | var  n    => n
+    | .not e    => s!"(! {expToString e})"
+    | app  n es => s!"({n} {unfoldExpressions es})"
+    | add  l r  => s!"({expToString l} + {expToString r})"
+    | mul  l r  => s!"({expToString l} * {expToString r})"
+    | eq   l r  => s!"({expToString l} = {expToString r})"
+    | ne   l r  => s!"({expToString l} != {expToString r})"
+    | lt   l r  => s!"({expToString l} < {expToString r})"
+    | le   l r  => s!"({expToString l} <= {expToString r})"
+    | gt   l r  => s!"({expToString l} > {expToString r})"
+    | ge   l r  => s!"({expToString l} >= {expToString r})"
 
   partial def progToStringAux (l : Nat) : Program → String
-    | skip => s!"{nSpaces l}skip"
-    | sequence p q => s!"{nSpaces (l-2)}{progToStringAux l p}\n{progToStringAux l q}"
-    | attribution n p =>
-      let pString := if p.length > 1 then s!"\n{progToStringAux (l+2) p}" else s!" {progToStringAux (l-2) p}"
+    | skip              => s!"{blank l}skip"
+    | sequence    p q   =>
+      s!"{blank (l-2)}{progToStringAux l p}\n{progToStringAux l q}"
+    | attribution n p   =>
+      let pString := if p.isSequence
+        then s!"\n{progToStringAux (l+2) p}"
+        else s!" {progToStringAux (l-2) p}"
       match p.getCurryNames? with
-      | none    => s!"{nSpaces l}{n} :=" ++ pString
-      | some ns => s!"{nSpaces l}{n} {ns.toList.unfoldStrings} :=" ++ pString
-    | evaluation e => s!"{nSpaces l}{expToString e}"
-    | whileLoop e p => s!"{nSpaces l}while {expToString e} do\n{progToStringAux (l+2) p}"
-    | ifElse e p q =>
-      s!"{nSpaces l}if {expToString e} then\n{progToStringAux (l+2) p}\nelse\n{progToStringAux (l+2) q}"
-    | err s => s
+      | none    => s!"{blank l}{n} :=" ++ pString
+      | some ns => s!"{blank l}{n} {ns.toList.unfoldStrings} :=" ++ pString
+    | evaluation  e     => s!"{blank l}{expToString e}"
+    | whileLoop   e p   =>
+      s!"{blank l}while {expToString e} do\n{progToStringAux (l+2) p}"
+    | ifElse      e p q =>
+      s!"{blank l}if {expToString e} then\n{progToStringAux (l+2) p}\n" ++
+        s!"else\n{progToStringAux (l+2) q}"
+    | fail        s     => s
 
   partial def progToString (p : Program) : String :=
     progToStringAux 0 p
 
 end
 
-instance : ToString Value      := ⟨valToString⟩
-instance : ToString Expression := ⟨expToString⟩
-instance : ToString Program    := ⟨progToString⟩
+def Value.toString      (v : Value)      : String := valToString  v
+def Expression.toString (e : Expression) : String := expToString  e
+def Program.toString    (p : Program)    : String := progToString p
 
-abbrev Context := Std.HashMap String Value
+instance : ToString Value      := ⟨toString⟩
+instance : ToString Expression := ⟨toString⟩
+instance : ToString Program    := ⟨toString⟩
 
-protected def Context.toString (c : Context) : String :=
-  (c.toList.foldl (init := "")
-    fun acc (n, val) => acc ++ s!"{n}:\t{val}\n").trimRight
+def Program.lengthAux (n : Nat) : Program → Nat
+  | Program.sequence _ p => p.lengthAux (n + 1)
+  | _                    => n + 1
 
-instance : ToString Context := ⟨Context.toString⟩
+def Program.length (p : Program) : Nat :=
+  p.lengthAux 0
 
 def Value.add : Value → Value → Value
-  | bool  bL, bool  bR => bool  $ bL || bR
-  | str   sL, str   sR => str   $ sL ++ sR
-  | int   iL, int   iR => int   $ iL +  iR
-  | float fL, float fR => float $ fL +  fR
-  | list  lL, list  lR => list  $ lL ++ lR
-  | _,        _        => error "invalid application of '+'"
+  | error s,     _           => error s
+  | _,           error s     => error s
+  | bool  bL,    bool  bR    => bool  $ bL || bR
+  | str   sL,    str   sR    => str   $ sL ++ sR
+  | int   iL,    int   iR    => int   $ iL +  iR
+  | float fL,    float fR    => float $ fL +  fR
+  | list  lL,    list  lR    => list  $ lL ++ lR
+  | list  lL,    vR          => list  $ lL.push vR
+  | curry nsL p, curry nsR q => curry (nsL.append nsR) (sequence p q)
+  | l,           r           =>
+    error s!"invalid application of '+' between\n{l}\nand\n{r}"
 
 def Value.mul : Value → Value → Value
+  | error s,  _        => error s
+  | _,        error s  => error s
   | bool  bL, bool  bR => bool  $ bL && bR
   | int   iL, int   iR => int   $ iL *  iR
   | float fL, float fR => float $ fL *  fR
-  | _,        _        => error "invalid application of '*'"
+  | curry .., curry .. => error "can't multiply programs"
+  | l,        r        =>
+    error s!"invalid application of '*' between\n{l}\nand\n{r}"
+
+def Value.lt : Value → Value → Value
+  | error s,   _         => error s
+  | _,         error s   => error s
+  | str   sL,  str   sR  => bool $ sL < sR
+  | int   iL,  int   iR  => bool $ iL < iR
+  | float fL,  float fR  => bool $ fL < fR
+  | list  lL,  list  lR  => bool $ lL.size < lR.size
+  | curry _ p, curry _ q => bool $ p.length < q.length
+  | l,         r         =>
+    error s!"invalid application of '<' between\n{l}\nand\n{r}"
+
+def Value.le : Value → Value → Value
+  | error s,   _         => error s
+  | _,         error s   => error s
+  | str   sL,  str   sR  => bool $ sL < sR || sL == sR
+  | int   iL,  int   iR  => bool $ iL ≤ iR
+  | float fL,  float fR  => bool $ fL ≤ fR
+  | list  lL,  list  lR  => bool $ lL.size ≤ lR.size
+  | curry _ p, curry _ q => bool $ p.length ≤ q.length
+  | l,         r         =>
+    error s!"invalid application of '<=' between\n{l}\nand\n{r}"
+
+def Value.gt : Value → Value → Value
+  | error s,   _         => error s
+  | _,         error s   => error s
+  | str   sL,  str   sR  => bool $ sL > sR
+  | int   iL,  int   iR  => bool $ iL > iR
+  | float fL,  float fR  => bool $ fL > fR
+  | list  lL,  list  lR  => bool $ lL.size > lR.size
+  | curry _ p, curry _ q => bool $ p.length > q.length
+  | l,         r         =>
+    error s!"invalid application of '>' between\n{l}\nand\n{r}"
+
+def Value.ge : Value → Value → Value
+  | error s,   _         => error s
+  | _,         error s   => error s
+  | str   sL,  str   sR  => bool $ sL > sR || sL == sR
+  | int   iL,  int   iR  => bool $ iL ≥ iR
+  | float fL,  float fR  => bool $ fL ≥ fR
+  | list  lL,  list  lR  => bool $ lL.size ≥ lR.size
+  | curry _ p, curry _ q => bool $ p.length ≥ q.length
+  | l,         r         =>
+    error s!"invalid application of '<=' between\n{l}\nand\n{r}"
 
 partial def Value.eq : Value → Value → Value
-  | bool  bL, bool  bR => bool $ bL = bR
-  | str   sL, str   sR => bool $ sL = sR
-  | int   iL, int   iR => bool $ iL = iR
+  | error s,   _       => error s
+  | _,         error s => error s
+  | nil,      nil      => bool true
+  | bool  bL, bool  bR => bool $ bL =  bR
+  | str   sL, str   sR => bool $ sL =  sR
+  | int   iL, int   iR => bool $ iL =  iR
   | float fL, float fR => bool $ fL == fR
   | list  lL, list  lR => bool $
     if lL.size = lR.size then
       lL.zip lR |>.foldl (init := true) $ fun acc (l, r) =>
         acc && match l.eq r with | bool true => true | _ => false
     else false
+  | curry .., curry .. => error "can't compare functions"
   | _,        _        => bool false
 
 partial def Value.ne : Value → Value → Value
+  | error s,   _       => error s
+  | _,         error s => error s
+  | nil,      nil      => bool false
   | bool  bL, bool  bR => bool $ bL ≠ bR
   | str   sL, str   sR => bool $ sL ≠ sR
   | int   iL, int   iR => bool $ iL ≠ iR
@@ -183,78 +275,57 @@ partial def Value.ne : Value → Value → Value
       lL.zip lR |>.foldl (init := false) $ fun acc (l, r) =>
         acc || match l.ne r with | bool true => true | _ => false
     else true
+  | curry .., curry .. => error "can't compare functions"
   | _,        _        => bool true
 
-def Value.lt : Value → Value → Value
-  | str   sL, str   sR => bool $ sL < sR
-  | int   iL, int   iR => bool $ iL < iR
-  | float fL, float fR => bool $ fL < fR
-  | list  lL, list  lR => bool $ lL.size < lR.size
-  | _,        _        => error "invalid application of '<'"
+def cantEvalAsBool (v : Value) : String :=
+  s!"can't evaluate as bool:\n{v}"
 
-def Value.le : Value → Value → Value
-  | str   sL, str   sR => bool $ sL < sR || sL == sR
-  | int   iL, int   iR => bool $ iL ≤ iR
-  | float fL, float fR => bool $ fL ≤ fR
-  | list  lL, list  lR => bool $ lL.size ≤ lR.size
-  | _,        _        => error "invalid application of '<='"
-
-def Value.gt : Value → Value → Value
-  | str   sL, str   sR => bool $ sL > sR
-  | int   iL, int   iR => bool $ iL > iR
-  | float fL, float fR => bool $ fL > fR
-  | list  lL, list  lR => bool $ lL.size > lR.size
-  | _,        _        => error "invalid application of '>'"
-
-def Value.ge : Value → Value → Value
-  | str   sL, str   sR => bool $ sL > sR || sL == sR
-  | int   iL, int   iR => bool $ iL ≥ iR
-  | float fL, float fR => bool $ fL ≥ fR
-  | list  lL, list  lR => bool $ lL.size ≥ lR.size
-  | _,        _        => error "invalid application of '>='"
-
-def cantEvalAsBool (v : Value) := s!"can't evaluate {v} as boolean"
-
+open NEList in
 def consume (p : Program) :
     NEList String → NEList Expression → (Option (NEList String)) × Program
-  | NEList.cons n ns, NEList.cons e es =>
+  | cons n ns, cons e es =>
     consume (sequence (attribution n (evaluation e)) p) ns es
-  | NEList.cons n ns, NEList.uno e     =>
-    (some ns, sequence (attribution n (evaluation e)) p)
-  | NEList.uno n,     NEList.uno e     =>
-    (none, sequence (attribution n (evaluation e)) p)
-  | NEList.uno _,     NEList.cons _ _  =>
-    (none, err "incompatible number of parameters")
+  | cons n ns, uno  e    => (some ns, sequence (attribution n (evaluation e)) p)
+  | uno  n,    uno  e    => (none, sequence (attribution n (evaluation e)) p)
+  | uno  _,    cons _ _  => (none, fail "incompatible number of parameters")
+
+abbrev Context := Std.HashMap String Value
+
+protected def Context.toString (c : Context) : String :=
+  (c.toList.foldl (init := "")
+    fun acc (n, val) => acc ++ s!"{n}:\t{val}\n").trimRight
+
+instance : ToString Context := ⟨Context.toString⟩
 
 mutual
 
   partial def evaluate (ctx : Context) : Expression → Value
-    | Expression.atom v    => v
-    | Expression.var n     => match ctx[n] with
+    | atom v     => v
+    | var  n     => match ctx[n] with
       | none   => error s!"'{n}' not found"
       | some v => v
-    | Expression.not e => match evaluate ctx e with
-      | Value.bool b => bool !b
-      | v            => error $ cantEvalAsBool v
-    | Expression.add eL eR => (evaluate ctx eL).add $ evaluate ctx eR
-    | Expression.mul eL eR => (evaluate ctx eL).mul $ evaluate ctx eR
-    | Expression.app n es  => match ctx[n] with
-      | none   => error s!"'{n}' not found"
-      | some v => match v with
-        | curry ns p =>
-          let (ns?, p') := consume p ns es
-          match ns? with
-          | none => (p'.run ctx).2 -- actually executing the function program
-          | some ns => curry ns p' -- there are still arguments to be fulfille
-        | _ => error s!"'{n}' is not a function"
-    | Expression.eq eL eR => (evaluate ctx eL).eq $ evaluate ctx eR
-    | Expression.ne eL eR => (evaluate ctx eL).ne $ evaluate ctx eR
-    | Expression.lt eL eR => (evaluate ctx eL).lt $ evaluate ctx eR
-    | Expression.le eL eR => (evaluate ctx eL).le $ evaluate ctx eR
-    | Expression.gt eL eR => (evaluate ctx eL).gt $ evaluate ctx eR
-    | Expression.ge eL eR => (evaluate ctx eL).ge $ evaluate ctx eR
+    | .not e => match evaluate ctx e with
+      | .bool b => bool !b
+      | v       => error $ cantEvalAsBool v
+    | .add eL eR => (evaluate ctx eL).add $ evaluate ctx eR
+    | .mul eL eR => (evaluate ctx eL).mul $ evaluate ctx eR
+    | app  n  es => match ctx[n] with
+      | none              => error s!"'{n}' not found"
+      | some (curry ns p) =>
+        let (ns?, p') := consume p ns es
+        match ns? with
+        | none    => (p'.run ctx).2 -- actually executing the function program
+        | some ns => curry ns p' -- there are still arguments to be fulfille
+      | _                 => error s!"'{n}' is not a function"
+    | .eq eL eR  => (evaluate ctx eL).eq $ evaluate ctx eR
+    | .ne eL eR  => (evaluate ctx eL).ne $ evaluate ctx eR
+    | .lt eL eR  => (evaluate ctx eL).lt $ evaluate ctx eR
+    | .le eL eR  => (evaluate ctx eL).le $ evaluate ctx eR
+    | .gt eL eR  => (evaluate ctx eL).gt $ evaluate ctx eR
+    | .ge eL eR  => (evaluate ctx eL).ge $ evaluate ctx eR
 
-  partial def Program.run (ctx : Context) : Program → Context × Value
+  partial def Program.run (ctx : Context := default) : Program → Context × Value
     | skip           => (ctx, nil)
     | sequence p₁ p₂ =>
       let res := p₁.run ctx
@@ -274,6 +345,6 @@ mutual
         (Program.whileLoop e p).run (p.run ctx).1
       | v            => (ctx, error $ cantEvalAsBool v)
     | evaluation e   => (ctx, (evaluate ctx e))
-    | err s          => (ctx, error s)
+    | fail s         => (ctx, error s)
 
 end
