FunnyLang/Meta.lean
@@ -1,0 +1,83 @@
+/-
+  Copyright (c) 2022 Arthur Paulino. All rights reserved.
+  Released under Apache 2.0 license as described in the file LICENSE.
+  Authors: Arthur Paulino
+-/
+
+import Lean
+import FunnyLang.AST
+import FunnyLang.Syntax
+
+open Lean Elab Meta
+
+def mkApp' (name : Name) (e : Expr) : Expr :=
+  mkApp (mkConst name) e
+
+def elabValue : Syntax → TermElabM Expr
+  | `(value|$n:numLit) =>
+    mkAppM ``Value.int #[mkApp' `Int.ofNat (mkNatLit n.toNat)]
+  | _ => throwUnsupportedSyntax
+
+def elabStringOfIdent (id : Syntax) : Expr :=
+  mkStrLit id.getId.toString
+
+partial def elabExpression : Syntax → TermElabM Expr
+  | `(expression| $v:value) => do mkAppM ``Expression.atom #[← elabValue v]
+  | `(expression| ! $e:expression) => do
+    mkAppM ``Expression.not #[← elabExpression e]
+  | `(expression| $n:ident $[$es:expression]*) => do
+    let es := (← es.mapM elabExpression).data
+    if h : ¬ es.isEmpty then -- fix: make an expression for `es.toNEList h`
+      let eh? := mkConst `sorry
+      mkAppM ``Expression.app #[elabStringOfIdent n, eh?]
+    else mkAppM ``Expression.var #[elabStringOfIdent n]
+  | `(expression| $l:expression + $r:expression) => do
+    mkAppM ``Expression.add #[← elabExpression l, ← elabExpression r]
+  | `(expression| $l:expression * $r:expression) => do
+    mkAppM ``Expression.mul #[← elabExpression l, ← elabExpression r]
+  | `(expression| $l:expression = $r:expression) => do
+    mkAppM ``Expression.eq #[← elabExpression l, ← elabExpression r]
+  | `(expression| $l:expression != $r:expression) => do
+    mkAppM ``Expression.ne #[← elabExpression l, ← elabExpression r]
+  | `(expression| $l:expression < $r:expression) => do
+    mkAppM ``Expression.lt #[← elabExpression l, ← elabExpression r]
+  | `(expression| $l:expression <= $r:expression) => do
+    mkAppM ``Expression.le #[← elabExpression l, ← elabExpression r]
+  | `(expression| $l:expression > $r:expression) => do
+    mkAppM ``Expression.gt #[← elabExpression l, ← elabExpression r]
+  | `(expression| $l:expression >= $r:expression) => do
+    mkAppM ``Expression.ge #[← elabExpression l, ← elabExpression r]
+  | `(expression| ($e:expression)) => elabExpression e
+  | _ => throwUnsupportedSyntax
+
+partial def elabProgram : Syntax → TermElabM Expr
+  | `(program| skip) => return mkConst ``Program.skip
+  | `(program| $p:program; $q:program) => do
+    mkAppM ``Program.sequence #[← elabProgram p, ← elabProgram q]
+  | `(program| $n:ident $ns:ident* := $p:program) => do
+    let ns := (ns.map elabStringOfIdent).data
+    if h : ¬ ns.isEmpty then
+      -- fix: make an expression for `ns.toNEList h`
+      let eh? := mkConst `sorry
+      mkAppM ``Program.attribution #[
+        elabStringOfIdent n,
+        mkApp' ``Program.evaluation $
+          mkApp' ``Expression.atom $
+            ← mkAppM ``Value.curry #[eh?, ← elabProgram p]
+      ]
+      else mkAppM ``Program.attribution #[elabStringOfIdent n, ← elabProgram p]
+  | `(program| if $e:expression then $p:program else $q:program) => do
+    mkAppM ``Program.ifElse
+      #[← elabExpression e, ← elabProgram p, ← elabProgram q]
+  | `(program| while $e:expression do $p:program) => do
+    mkAppM ``Program.whileLoop #[← elabExpression e, ← elabProgram p]
+  | `(program| $e:expression) => do
+    mkAppM ``Program.evaluation #[← elabExpression e]
+  | `(program| ($p:program)) => elabProgram p
+  | _ => throwUnsupportedSyntax
+
+elab ">>" ppLine p:program ppLine "<<" : term => elabProgram p
+
+#eval >>
+x := 2; x = x
+<<.run
