FunnyLang/Syntax.lean
@@ -1,0 +1,37 @@
+/-
+  Copyright (c) 2022 Arthur Paulino. All rights reserved.
+  Released under Apache 2.0 license as described in the file LICENSE.
+  Authors: Arthur Paulino
+-/
+
+declare_syntax_cat                            value
+syntax ("-" noWs)? num                      : value
+syntax str                                  : value
+syntax "true"                               : value
+syntax "false"                              : value
+syntax ("-" noWs)? num noWs "." (noWs num)? : value
+syntax " [ " value* " ] "                   : value
+syntax "nil"                                : value
+
+declare_syntax_cat                    expression
+syntax value                        : expression
+syntax expression " + " expression  : expression
+syntax expression " * " expression  : expression
+syntax " ! " expression             : expression
+syntax expression " = " expression  : expression
+syntax expression " != " expression : expression
+syntax expression " < " expression  : expression
+syntax expression " <= " expression : expression
+syntax expression " > " expression  : expression
+syntax expression " >= " expression : expression
+syntax ident expression*            : expression
+syntax " ( " expression " ) "       : expression
+
+declare_syntax_cat                                     program
+syntax "skip"                                        : program
+syntax:25 program " ; " program                      : program
+syntax ident+ " := " program:75                      : program
+syntax expression                                    : program
+syntax "if" expression "then" program "else" program : program
+syntax "while" expression "do" program               : program
+syntax " ( " program " ) "                           : program
